coq_session_new/eproc_sr.v
@@ -1,6 +1,6 @@
 From mathcomp Require Import ssreflect ssrbool eqtype ssrnat seq zify.
 From Coq Require Import ssrfun Classical Utf8.
-Require Export AutosubstSsr ARS proc_sr eproc_occurs.
+Require Export AutosubstSsr ARS era_inv proc_sr eproc_occurs.
 
 Set Implicit Arguments.
 Unset Strict Implicit.
@@ -8,13 +8,115 @@ Unset Printing Implicit Defensive.
 
 Lemma eproc_congr0_type Θ p p' q :
   proc_congr0 p q -> Θ ⊢ p ~ p' -> exists2 q', proc_congr0 p' q' & Θ ⊢ q ~ q'.
-Proof with eauto using proc_type, proc_congr0.
-Admitted.
+Proof with eauto using era_type, eproc_type, proc_congr0.
+  move=>cgr. elim: cgr Θ p'=>{p q}.
+  { move=>p q Θ p' er. inv er.
+    exists (q' ∣ p'0)...
+    econstructor.
+    apply: merge_sym...
+    all: eauto. }
+  { move=>o p q Θ p' er. inv er. inv H5.
+    have[Θ4[mrg1 mrg2]]:=merge_splitL (merge_sym H1) H2.
+    exists ((p'0 ∣ p') ∣ q'0)...
+    econstructor. apply: mrg2.
+    econstructor. apply: merge_sym.
+    all: eauto. }
+  { move=>p q Θ p' er. inv er. inv H3.
+    exists (ν.(p' ∣ proc_cren q' (+2))).
+    constructor.
+    move: H4. move e:(~~r2)=>r1 erp.
+    econstructor. apply: (esym e).
+    econstructor.
+    2:{ apply: erp. }
+    2:{ replace (proc_cren q (+2)) with (proc_cren (proc_cren q (+1)) (+1)).
+        replace (proc_cren q' (+2)) with (proc_cren (proc_cren q' (+1)) (+1)).
+        apply: eproc_cweaken.
+        apply: eproc_cweaken.
+        apply: H5.
+        rewrite<-proc_cren_comp. by asimpl.
+        rewrite<-proc_cren_comp. by asimpl. }
+    repeat constructor... }
+  { move=>p p' q q' cgr1 ih1 cgr2 ih2 Θ p0 er. inv er.
+    have[p1 cgr3 erp]:=ih1 _ _ H3.
+    have[q1 cgr4 erq]:=ih2 _ _ H5.
+    exists (p1 ∣ q1)... }
+  { move=>p p' cgr ih Θ p0 er. inv er.
+    have[p1 cgr1 erp]:=ih _ _ H2.
+    exists (ν.p1)... }
+  { move=>p Θ p' er. inv er. inv H5.
+    have[n e]:=era_return_form H2. subst.
+    have er:=era_return_inv H2.
+    have e:=era_ii_form er. subst.
+    have emp:=era_ii_inv er.
+    have e:=merge_emptyR H1 emp. subst... }
+Qed.
 
 Lemma eproc_congr0_typei Θ p q q' :
   proc_congr0 p q -> Θ ⊢ q ~ q' -> exists2 p', proc_congr0 p' q' & Θ ⊢ p ~ p'.
-Proof with eauto using proc_type, proc_congr0.
-Admitted.
+Proof with eauto using era_type, eproc_type, proc_congr0.
+  move=>cgr. elim: cgr Θ q'=>{p q}.
+  { move=>p q Θ q' er. inv er.
+    exists (q'0 ∣ p'). constructor.
+    econstructor.
+    apply: merge_sym...
+    all: eauto. }
+  { move=>o p q Θ q' er. inv er. inv H3.
+    have[Θ4[mrg1 mrg2]]:=merge_splitR H1 H2.
+    exists (p'0 ∣ (q' ∣ q'0)). apply: proc_congr0_assoc.
+    econstructor.
+    apply: merge_sym.
+    apply: mrg2.
+    eauto.
+    econstructor... }
+  { move=>p q Θ q' er. inv er. inv H2. inv H1; inv H3.
+    { have[q0 e]:=eproc_cren_inv H6. subst.
+      replace (proc_cren q (+2))
+        with (proc_cren (proc_cren q (+1)) (+1)) in H6.
+      replace (proc_cren q0 (+2))
+        with (proc_cren (proc_cren q0 (+1)) (+1)) in H6.
+      have erq:=eproc_cstrengthen (eproc_cstrengthen H6).
+      exists (ν.p'0 ∣ q0).
+      constructor.
+      econstructor...
+      rewrite<-proc_cren_comp. by asimpl.
+      rewrite<-proc_cren_comp. by asimpl. }
+    { have[q0 e]:=eproc_cren_inv H6. subst.
+      have:=eproc_occurs_iren H6 iren1.
+      have[->_]:proc_occurs 1 (proc_cren q (+2)) = 1 ∧
+               proc_occurs 1 (proc_cren q0 (+2)) = 1.
+      apply: eproc_type_occurs1...
+      repeat constructor.
+      by move=>[]. }
+    { have[q0 e]:=eproc_cren_inv H6. subst.
+      have:=eproc_occurs_iren H6 iren0.
+      have[->_]:proc_occurs 0 (proc_cren q (+2)) = 1 ∧
+               proc_occurs 0 (proc_cren q0 (+2)) = 1.
+      apply: eproc_type_occurs1...
+      repeat constructor.
+      by move=>[]. }
+    { have[q0 e]:=eproc_cren_inv H6. subst.
+      have:=eproc_occurs_iren H6 iren0.
+      have[->_]:proc_occurs 0 (proc_cren q (+2)) = 1 ∧
+               proc_occurs 0 (proc_cren q0 (+2)) = 1.
+      apply: eproc_type_occurs1...
+      repeat constructor.
+      by move=>[]. } }
+  { move=>p p' q q' cgr1 ih1 crg2 ih2 Θ q0 er. inv er.
+    have[p2 cgr3 erp]:=ih1 _ _ H3.
+    have[q2 cgr4 erq]:=ih2 _ _ H5.
+    exists (p2 ∣ q2)... }
+  { move=>p p' cgr ih Θ q' er. inv er.
+    have[p1 cgr1 erp]:=ih _ _ H2.
+    exists (ν.p1)... }
+  { move=>p Θ q' er.
+    have wf:=eproc_type_wf er.
+    have[Θ0[emp mrg]]:=proc_wf_empty wf.
+    exists (q' ∣ ⟨ Return II ⟩)...
+    econstructor.
+    apply: merge_sym.
+    all: eauto.
+    repeat constructor... }
+Qed.
 
 Lemma eproc_congr_type Θ p p' q :
   p ≡ q -> Θ ⊢ p ~ p' -> exists2 q', p' ≡ q' & Θ ⊢ q ~ q'.
